rywu: fix proof

theories/examples/run_yield_with_unknown/proof.v
@@ -1,16 +1,15 @@
 From machine_program_logic.program_logic Require Import weakestpre.
-From HypVeri.algebra Require Import base.
+From HypVeri.algebra Require Import base lower_bound.
 From HypVeri.rules Require Import rules_base mov halt run yield.
 From HypVeri.examples Require Import instr.
 From HypVeri.logrel Require Import logrel.
-From HypVeri Require Import proofmode.
+From HypVeri Require Import proofmode machine_extra.
 Require Import Setoid.
 
 Program Instance rywu_vmconfig : HypervisorConstants :=
     {vm_count := 3;
      vm_count_pos:= _}.
 
-Program Definition V0 : VMID := (@nat_to_fin 0 _ _).
 Program Definition V1 : VMID := (@nat_to_fin 1 _ _).
 Program Definition V2 : VMID := (@nat_to_fin 2 _ _).
 
@@ -37,22 +36,25 @@ Section proof.
 
   Context `{!gen_VMG Σ}.
 
-  (* TODO *)
-  Lemma rywu_machine0 {prog1page} R :
-      let Q := ((* R0 & R1 of pvm *)
-        (R0 @@ V0 ->r encode_hvc_func(Run) ∗ R1 @@ V0 ->r encode_vmid(V2)))%I in
+  Notation VMProp2 ps p:= (VMProp_unknown V2 ps p ∅) (only parsing).
+
+  Lemma rywu_machine0 {prog1page prog3page} p_rx2 :
+      let R2 := (RX@V2 :=() ∗ RX@ V2 := p_rx2 ∗ memory_cells {[p_rx2]})%I in
+      prog1page ≠ prog3page ->
       seq_in_page (of_pid prog1page) (length rywu_program1) prog1page ->
-      R ∗
-      (program (rywu_program1) (of_pid prog1page)) ∗ (VMProp V0 True%I 1) ∗
-      (VMProp V1 ((R0 @@ V0 ->r run_I ∗ R1 @@ V0 ->r encode_vmid V1 ) ∗
-                    VMProp V0 ((R0 @@ V0 ->r yield_I ∗ R1 @@ V0 ->r encode_vmid V1 ) ∗
-                                 VMProp V1 False%I (1/2)%Qp) (1/2)%Qp)%I (1/2)%Qp) ∗
-      (VMProp V2 (Q ∗ VMProp V0 ((R0 @@ V0 ->r yield_I ∗ R1 @@ V0 ->r encode_vmid V2 ∗
-                                  (R )) ∨ False) (1/2)%Qp) (1/2%Qp)) ∗
+      (program (rywu_program1) (of_pid prog1page)) ∗
       (V0 -@A> [{[prog1page]}]) ∗
       (PC @@ V0 ->r (of_pid prog1page)) ∗
       (∃ r0, R0 @@ V0 ->r r0) ∗
-      (∃ r1, R1 @@ V0 ->r r1)
+      (∃ r1, R1 @@ V0 ->r r1) ∗
+      (VMProp V0 True%I 1) ∗
+      (VMProp V1 ((R0 @@ V0 ->r run_I ∗ R1 @@ V0 ->r encode_vmid V1) ∗
+                    VMProp V0 ((R0 @@ V0 ->r yield_I ∗ R1 @@ V0 ->r encode_vmid V1) ∗
+                                 VMProp V1 False%I (1/2)%Qp) (1/2)%Qp)%I (1/2)%Qp) ∗
+      (VMProp2 {[prog3page]} p_rx2) ∗
+      LB_auth ∅ ∗
+      hp [hs_all] ∗
+      R2
       ⊢ WP ExecI @ V0
             {{ (λ m,
                  ⌜m = HaltI⌝ ∗
@@ -60,100 +62,121 @@ Section proof.
                  (V0 -@A> [{[prog1page]}]) ∗
                  PC @@ V0 ->r ((of_pid prog1page) ^+ (length rywu_program1))%f∗
                  R0 @@ V0 ->r yield_I ∗
-                 R1 @@ V0 ->r encode_vmid V2 ∗
-                 R)}}%I.
+                 R1 @@ V0 ->r encode_vmid V2
+                 )}}%I.
   Proof.
-    iIntros (Q HIn) "(R & Q & (p_1 & p_2 & p_3 & p_4 & p_5 & p_6 & p_7 & _) & Hprop0 & Hprop1 & Hprop2 & Hacc & Hacc' & PCz & R0z & R1z)".
+    rewrite /VMProp_unknown.
+    iIntros (Hneq_p HIn) "((p_1 & p_2 & p_3 & p_4 & p_5 & p_6 & p_7 & _) & acc & PCz & (%r0 & R0z) & (%r1 & R1z)
+                            & prop0 & prop1 & prop2 & LB_auth & hp & R2)".
     pose proof (seq_in_page_forall2 _ _ _ HIn) as Hforall.
     clear HIn; rename Hforall into HIn.
-    iDestruct "R0z" as "(%r0 & R0z)".
-    iDestruct "R1z" as "(%r1 & R1z)".
     (* mov_word_I R0 run_I *)
     rewrite wp_sswp.
-    iApply ((mov_word (of_pid prog1page) run_I R0) with "[p_1 PCz Hacc R0z]");try rewrite HIn //; iFrameAutoSolve; try set_solver +.
+    iApply ((mov_word (of_pid prog1page) run_I R0) with "[p_1 PCz acc R0z]");try rewrite HIn //; iFrameAutoSolve; try set_solver +.
     iModIntro.
-    iIntros "(PCz & p_1 & Hacc & R0z)".
-    iIntros "_".
+    iIntros "(PCz & p_1 & acc & R0z) _".
     (* mov_word_I R1 V1 *)
     rewrite wp_sswp.
-    iApply ((mov_word ((of_pid prog1page) ^+ 1)%f (encode_vmid V1) R1) with "[p_2 PCz Hacc R1z]"); try rewrite HIn //; iFrameAutoSolve; try set_solver +.
+    iApply ((mov_word ((of_pid prog1page) ^+ 1)%f (encode_vmid V1) R1) with "[p_2 PCz acc R1z]"); try rewrite HIn //; iFrameAutoSolve; try set_solver +.
     iModIntro.
-    iIntros "(PCz & p_2 & Hacc & R1z)".
-    iIntros "_".
+    iIntros "(PCz & p_2 & acc & R1z) _".
     (* hvc_I *)
     rewrite wp_sswp.
-    set (T := (PC @@ V0 ->r (((prog1page ^+ 1) ^+ 1) ^+ 1)%f ∗ ((prog1page ^+ 1) ^+ 1)%f ->a hvc_I ∗ prog1page -@A> V0)%I).
-    iApply ((run (((of_pid prog1page) ^+ 1) ^+ 1)%f V1 (s:= {[V0]}) (R := (prog2page -@A> V1)%I) (R' := T) (i' := 1))
-             with "[PCz p_3 Hacc Hacc' R0z R1z Hprop0 Hprop1]"); try rewrite HIn //;iFrameAutoSolve.
-    { set_solver +. }
+    set (T := (PC @@ V0 ->r (((prog1page ^+ 1) ^+ 1) ^+ 1)%f ∗ ((prog1page ^+ 1) ^+ 1)%f ->a hvc_I ∗ V0 -@A> [{[prog1page]}])%I).
+    iApply ((run (((of_pid prog1page) ^+ 1) ^+ 1)%f V1 (R := True) (R' := T) (i' := 1))
+             with "[PCz p_3 acc R0z R1z prop0 prop1]"); try rewrite HIn //;iFrameAutoSolve.
     { solve_finz. }
     { solve_finz. }
     { apply decode_encode_hvc_func. }
     { apply decode_encode_vmid. }
     {
-      iSplitR "Hprop0".
+      iSplitR "prop0".
       - iModIntro.
-        iFrame "Hprop1".
-      - iSplitL "Hprop0".
-        iFrame "Hprop0".
+        iFrame "prop1".
+      - iSplitL "prop0".
+        iFrame "prop0".
+        iSplitR "";last done.
         iNext.
-          iIntros "[(PCz & p_4 & Hacc & R0z & R1z) R]".
-          iFrame.
+        iIntros "[(PCz & p_4 & acc & R0z & R1z) _]".
+        iFrame.
     }
-    {
-    set_solver.
-    }
+    { set_solver. }
     iModIntro.
-    subst T.
-    iIntros "[(PC & p_3 & Hacc) Hprop0] Hholds".
-    iDestruct (VMProp_holds_agree with "[Hholds Hprop0]") as "[P' Hprop0]".
-    iFrame "Hprop0".
-    iSimpl.
-    iSimpl in "Hholds".
-    done.
+    iIntros "[(PC & p_3 & acc) prop0] Hholds".
+    iDestruct (VMProp_holds_agree with "[Hholds prop0]") as "[P' prop0]".
+    iFrame "prop0".
+    iFrame.
     (* getting back resources *)
-    iDestruct "P'" as "((>R0z & >R1z & >Hacc') & Hprop1)".
+    iDestruct "P'" as "((>R0z & >R1z) & prop1)".
     rewrite wp_sswp.
-    iApply ((mov_word _ run_I R0) with "[p_4 PC Hacc R0z]");try rewrite HIn //; iFrameAutoSolve; try set_solver +.
+    iApply ((mov_word _ run_I R0) with "[p_4 PC acc R0z]");try rewrite HIn //; iFrameAutoSolve; try set_solver +.
     iModIntro.
-    iIntros "(PCz & p_4 & Hacc & R0z)".
+    iIntros "(PCz & p_4 & acc & R0z)".
     iIntros "_".
     (* mov_word_I R1 V2 *)
     rewrite wp_sswp.
-    iApply ((mov_word _ (encode_vmid V2) R1) with "[p_5 PCz Hacc R1z]"); try rewrite HIn //; iFrameAutoSolve; try set_solver +.
+    iApply ((mov_word _ (encode_vmid V2) R1) with "[p_5 PCz acc R1z]"); try rewrite HIn //; iFrameAutoSolve; try set_solver +.
     iModIntro.
-    iIntros "(PCz & p_5 & Hacc & R1z)".
-    iIntros "_".
+    iIntros "(PCz & p_5 & acc & R1z) _".
     (* hvc_I *)
+    iDestruct (lb_update_alloc V2 {[prog1page]} with "LB_auth") as ">[LB_auth LB2]";first done.
     rewrite wp_sswp.
-    set (R' := (PC @@ V0 ->r ((((((prog1page ^+ 1) ^+ 1) ^+ 1) ^+ 1) ^+ 1) ^+ 1)%f ∗
-            (((((prog1page ^+ 1) ^+ 1) ^+ 1) ^+ 1) ^+ 1)%f ->a hvc_I ∗
-                    prog1page -@A> V0)%I).
-    iApply ((run (((((prog1page ^+ 1) ^+ 1) ^+ 1) ^+ 1) ^+ 1)%f V2 (R := R%I)
+    iApply ((run (((((prog1page ^+ 1) ^+ 1) ^+ 1) ^+ 1) ^+ 1)%f V2 (R := True%I)
                 (R' := PC @@ V0 ->r ((((((prog1page ^+ 1) ^+ 1) ^+ 1) ^+ 1) ^+ 1) ^+ 1)%f
-                                 ∗(((((prog1page ^+ 1) ^+ 1) ^+ 1) ^+ 1) ^+ 1)%f ->a hvc_I )
-                (i' := 2)) with "[PCz p_6 Hacc Hacc' R0z R1z Hprop0 Hprop2 Q R]"); try rewrite HIn //;iFrameAutoSolve.
-    { set_solver +. }
+                                 ∗(((((prog1page ^+ 1) ^+ 1) ^+ 1) ^+ 1) ^+ 1)%f ->a hvc_I ∗ V0 -@A> [{[prog1page]}] )
+                (i' := 2)) with "[PCz p_6 acc R0z R1z prop0 prop2 LB2 hp R2]"); try rewrite HIn //;iFrameAutoSolve.
     { solve_finz. }
     { solve_finz. }
     { apply decode_encode_hvc_func. }
     { apply decode_encode_vmid. }
-    { iSplitL "Hprop2".
-      done.
-      iSplitL "Hprop0".
-      done.
-      iFrame "R".
-      iNext.
-      iIntros "((PC & addr & acc & R0 & R1) & R)".
-      iFrame "PC addr".
-      unfold Q.
+    { iSplitL "prop2".
       iFrame.
-      iApply "Q".
+      iSplitL "prop0".
+      done.
+      iSplitR "";last done.
+      iNext.
+      iIntros "((PC & addr & acc & R0 & R1) & _)".
+      iFrame "PC addr R0 R1 acc".
+      iExists {[prog1page]}, ∅, hs_all.
+      iFrame.
+      iSplitL "";first done.
+      iSplitL "".
+      { rewrite disjoint_singleton_l not_elem_of_singleton //. }
+      iSplitL "".
+      { iPureIntro.
+        rewrite /inv_trans_hpool_consistent'. split.
+        {
+          rewrite /inv_trans_hpool_disj dom_empty_L.
+          apply disjoint_empty_l.
+        }
+        {
+          rewrite /inv_finite_handles dom_empty_L union_empty_l_L //.
+        }
+      }
+      iSplitL "".
+      {
+        rewrite /transferred_tran_entries.
+        by iApply big_sepM_empty.
+      }
+      iSplitL "".
+      {
+        rewrite /transferred_pgt_entries.
+        by iApply big_sepM_empty.
+      }
+      iSplitL "".
+      {
+        rewrite /accessible_trans.
+        rewrite map_filter_empty.
+        rewrite /ps_trans map_fold_empty.
+        rewrite /memory_cells.
+        by iApply big_sepS_empty.
+      }
+      iDestruct "R2" as "(rx_s & rx & rx_mem)".
       iFrame.
     }
     { set_solver +. }
     iNext.
-    iIntros "((PC & p_6) & Hprop0) Hholds0".
+    iIntros "((PC & p_6 & acc) & Hprop0) Hholds0".
     iDestruct (VMProp_holds_agree with "[Hholds0 Hprop0]") as "[P' Hprop0]".
     iSplitR "Hprop0".
     2: { iFrame "Hprop0". }
@@ -161,7 +184,7 @@ Section proof.
     iSimpl in "Hholds0".
     done.
     (* getting back resources *)
-    iDestruct "P'" as "[(>R0z & >R1z & R & >acc)|>False]".
+    iDestruct "P'" as ">[(% & % & % & % & ? & ? & ? & ? & ? & ? & R0z & R1z)|False]".
     2: { (* V2 does not yield *)
     iExFalso.
     iExact "False".
@@ -189,17 +212,17 @@ Section proof.
   Lemma rywu_machine1 {prog2page} :
       seq_in_page (of_pid prog2page) (length rywu_program2) prog2page ->
       (program rywu_program2 (of_pid prog2page))
-        ∗ (VMProp V1 ((R0 @@ V0 ->r run_I ∗ R1 @@ V0 ->r encode_vmid V1 ∗ (prog2page -@A> V1))
-        ∗ VMProp V0 ((R0 @@ V0 ->r yield_I ∗ R1 @@ V0 ->r encode_vmid V1 ∗ (prog2page -@A> V1)) ∗ VMProp V1 False%I (1/2)%Qp) (1/2)%Qp)%I (1/2)%Qp)
+        ∗ (VMProp V1 ((R0 @@ V0 ->r run_I ∗ R1 @@ V0 ->r encode_vmid V1 )
+        ∗ VMProp V0 ((R0 @@ V0 ->r yield_I ∗ R1 @@ V0 ->r encode_vmid V1 ) ∗ VMProp V1 False%I (1/2)%Qp) (1/2)%Qp)%I (1/2)%Qp)
         ∗ (PC @@ V1 ->r (of_pid prog2page))
         ∗ (∃ r0, R0 @@ V1 ->r r0)
+        ∗ (V1 -@A> [{[prog2page]}] )
         ⊢ VMProp_holds V1 (1/2)%Qp -∗ (WP ExecI @ V1
               {{ (λ m, False)}}%I).
   Proof.
-    iIntros (HIn ) "((p_1 & p_2 & _) & HPropi & PC1 & R01)".
-    iIntros "HPropH".
-    iDestruct "R01" as "[%r0 R01]".
-    iDestruct (VMProp_holds_agree V1 with "[HPropH HPropi]") as "[Prop VMProp]".
+    iIntros (HIn ) "((p_1 & p_2 & _) & prop1 & PC1 & [%r0 R01] & acc)".
+    iIntros "Hholds".
+    iDestruct (VMProp_holds_agree V1 with "[Hholds prop1]") as "[P prop1]".
     iFrame.
     pose proof (seq_in_page_forall2 _ _ _ HIn) as Hforall.
     clear HIn; rename Hforall into HIn.
@@ -207,42 +230,37 @@ Section proof.
     by simpl.
     (* mov_word_I R0 yield_I *)    
     rewrite wp_sswp.
-    iDestruct "Prop" as "[(HRz0 & HRz1 & Hacc) VMPropz]".
-    iApply ((mov.mov_word (of_pid prog2page) yield_I R0) with "[p_1 PC1 Hacc R01]");try rewrite HIn //;iFrameAutoSolve;try set_solver.
-    { iFrame. }
+    iDestruct "P" as "[(R0z & R1z) prop0]".
+    iApply ((mov.mov_word (of_pid prog2page) yield_I R0) with "[p_1 PC1 acc R01]");try rewrite HIn //;iFrameAutoSolve;try set_solver.
     iModIntro.
-    iIntros "(PC1 & p_1 & Hacc & R0i)".
+    iIntros "(PC1 & p_1 & acc & R01)".
     iSimpl.
     rewrite HV1.
     iIntros "_".
     (* hvc_I *)
     rewrite wp_sswp.
-    iApply ((yield ((of_pid prog2page) ^+ 1)%f (z := V0) (Q := (R0 @@ V0 ->r yield_I ∗ R1 @@ V0 ->r encode_vmid V1 ∗ (prog2page -@A> V1))%I)
+    iApply ((yield ((of_pid prog2page) ^+ 1)%f (z := V0) (Q := (R0 @@ V0 ->r yield_I ∗ R1 @@ V0 ->r encode_vmid V1)%I)
                    (P' := False%I) (R := True%I) (i' := 1)
                    (R' := (PC @@ V1 ->r ((prog2page ^+ 1) ^+ 1)%f ∗ (prog2page ^+ 1)%f ->a hvc_I ∗ R0 @@ V1 ->r yield_I)%I))
-         with "[PC1 p_2 Hacc R0i HRz0 HRz1 VMPropz VMProp]"); try rewrite HIn //;iFrameAutoSolve.
-    { set_solver +. }
+         with "[PC1 p_2 acc R01 R0z R1z prop0 prop1]"); try rewrite HIn //;iFrameAutoSolve.
     { solve_finz. }
     { apply decode_encode_hvc_func. }
-    { iSplitL "VMPropz".
+    { iSplitL "prop0".
+      iFrame.
+      iSplitL "prop1".
+      iFrame.
+      iSplitL "";last done.
       iNext.
-      iFrame "VMPropz".
-      iSplitL "VMProp".
-      iNext.
-      iFrame "VMProp".
-      iSplitL "".
-      - iNext.
-        iIntros "[(? & ? & ? & ? & ? & ?) ?]".
-        iFrame.
-      - by iNext.
+      iIntros "[(? & ? & ? & ? & ? & ?) ?]".
+      iFrame.
     }
     { set_solver +. }
     iModIntro.
-    iIntros "[? VMProp] VMPropH".
+    iIntros "[? prop1] Hholds".
     simpl.
-    iDestruct (VMProp_holds_agree V1 with "[VMProp VMPropH]") as "[Prop VMProp]".
-    iFrame "VMProp VMPropH".
-    iMod "Prop".
+    iDestruct (VMProp_holds_agree V1 with "[prop1 Hholds]") as "[P prop1]".
+    iFrame.
+    iMod "P".
     by iExFalso.
   Qed.
   
