theories/logrel/logrel.v
@@ -1,6 +1,7 @@
 From iris.proofmode Require Import tactics.
 From machine_program_logic.program_logic Require Import weakestpre.
 From HypVeri.lang Require Import lang.
+From HypVeri Require Import machine_extra.
 From HypVeri.algebra Require Import base base_extra mem.
 Import uPred.
 
@@ -10,10 +11,6 @@ Section logrel.
   Context `{hypparams:!HypervisorParameters}.
   Context `{vmG: !gen_VMG Σ}.
 
-  Program Definition V0 : VMID := (@nat_to_fin 0 _ _).
-  Next Obligation.
-  destruct hypconst. simpl. lia.
-  Defined.
 
   (* XXX: a better def using list zip? - no, gmap makes case analysis simpler*)
   Definition unknown_mem_page (p: PID) :=
@@ -24,7 +21,7 @@ Section logrel.
   Context (i : (leibnizO VMID)).
 
   Program Definition interp_execute: iPropO Σ :=
-   (⌜ fin_to_nat i ≠ 0 ⌝ -∗
+   (⌜i ≠ V0⌝ -∗
         (VMProp_holds i (1/2)%Qp -∗ WP ExecI @ i {{(λ _, True )}}))%I.
 
   Definition pgt_entries_own_excl (ps: gset PID) (vo: VMID) (be:bool) : iProp Σ:=
@@ -32,7 +29,7 @@ Section logrel.
 
   (* [transferred_tran_entries] includes all transaction related entries transferred to/from i from/to primary when scheduling,*)
   Definition transferred_tran_entries (trans: gmap Addr transaction) : iProp Σ:=
-    [∗ map] h ↦ tran ∈ trans ,
+    [∗ map] h ↦ tran ∈ trans,
         (* All of half of transactions are required, as we don't know which one would be used by i.
           Only *half* is needed so that related vms can remember transactions by keeping the other half. *)
         h -{1/2}>t tran.1 ∗
@@ -67,6 +64,44 @@ Section logrel.
   Definition ps_trans (trans: gmap Word transaction) : gset PID :=
     map_fold (λ (k:Addr) v acc, v.1.1.2 ∪ acc) (∅: gset PID) trans.
 
+  Definition VMProp_unknown ps_acc p_rx trans :=
+    VMProp i (((∃ ps_na (trans' : gmap Word transaction) hpool,
+                    let ps_trans' := ps_trans (accessible_trans trans') in
+                    ⌜accessible_trans trans = accessible_trans trans'⌝ ∗
+                    (* lower bound *)
+                    LB@ i := [ps_na] ∗ ⌜ps_na ## ps_acc⌝ ∗
+                    (* we need this to ensure all transaction entries are transferred *)
+                    ⌜inv_trans_hpool_consistent' trans' hpool⌝ ∗
+                    (* transaction entries *)
+                    hp [hpool] ∗ transferred_tran_entries trans' ∗
+                    (* page table entries *)
+                    transferred_pgt_entries trans' ∗
+                    (* mem *)
+                    memory_cells ps_trans' ∗
+                    (* status of RX *)
+                    (RX@ i :=() ∨ ∃l s, RX@i :=(l,s)) ∗
+                    (* RX *)
+                    (RX@i := p_rx ∗ memory_cells {[p_rx]})) ∗
+                  R0 @@ V0 ->r encode_hvc_func(Run) ∗ R1 @@ V0 ->r encode_vmid(i)) ∗
+                  (* if i yielding, we give following resources back to pvm *)
+                  VMProp V0 (
+                           (∃ ps_na' ps_acc' trans'' hpool',
+                             (* TODO: we may need more constraints for trans'',
+                                      probably relate it to trans'(currently impossible because of the form of yield rule) *)
+                             let ps_trans'' := ps_trans (accessible_trans trans'') in
+                             (* lower bound *)
+                             LB@ i := [ps_na'] ∗ ⌜ps_na' ## ps_acc'⌝ ∗
+                                        (* resources *)
+                                        hp [hpool'] ∗ transferred_tran_entries trans'' ∗
+                                        transferred_pgt_entries trans'' ∗
+                                        memory_cells ps_trans'' ∗
+                                        (* R0 and R1 of pvm *)
+                                        R0 @@ V0 ->r encode_hvc_func(Yield) ∗ R1 @@ V0 ->r encode_vmid(i))
+                                      (* no scheduling, we finish the proof *)
+                                      (* NOTE: if i will be scheduled arbitrary number of times, need recursive definition *)
+                                      ∨ False) (1/2)%Qp)
+               (1/2)%Qp.
+
   Program Definition interp_access ps_acc p_tx p_rx (trans : gmap Word transaction) : iPropO Σ:=
     (
       let ps_nea := ps_trans (accessible_trans trans) ∪ {[p_rx]} in
@@ -85,41 +120,7 @@ Section logrel.
       (* mem *)
       memory_cells ps_ea ∗
       (* VMProp *)
-      VMProp i ((∃ ps_na (trans' : gmap Word transaction) hpool,
-                    let ps_trans' := ps_trans (accessible_trans trans') in
-                    ⌜accessible_trans trans = accessible_trans trans'⌝ ∗
-                    (* lower bound *)
-                    LB@ i := [ps_na] ∗ ⌜ps_na ## ps_acc⌝ ∗
-                    (* we need this to ensure all transaction entries are transferred *)
-                    ⌜inv_trans_hpool_consistent' trans' hpool⌝ ∗
-                    (* transaction entries *)
-                    hp [hpool] ∗ transferred_tran_entries trans' ∗
-                    (* page table entries *)
-                    transferred_pgt_entries trans' ∗
-                    (* mem *)
-                    memory_cells ps_trans' ∗
-                    (* status of RX *)
-                    (RX@ i :=() ∨ ∃l s, RX@i :=(l,s)) ∗
-                    (* RX *)
-                    (RX@i := p_rx ∗ memory_cells {[p_rx]})) ∗
-                  R0 @@ V0 ->r encode_hvc_func(Run) ∗ R1 @@ V0 ->r encode_vmid(i) ∗
-                  (* if i yielding, we give following resources back to pvm *)
-                  VMProp V0 (
-                           ∃ ps_na' ps_acc' trans'' hpool',
-                             let ps_trans'' := ps_trans (accessible_trans trans'') in
-                             (* lower bound *)
-                             LB@ i := [ps_na'] ∗ ⌜ps_na' ## ps_acc'⌝ ∗
-                                        (* resources *)
-                                        hp [hpool'] ∗ transferred_tran_entries trans'' ∗
-                                        transferred_pgt_entries trans'' ∗
-                                        memory_cells ps_trans'' ∗
-                                        (* R0 and R1 of pvm *)
-                                        (R0 @@ V0 ->r encode_hvc_func(Yield) ∗ R1 @@ V0 ->r encode_vmid(i))
-                                      (* no scheduling, we finish the proof *)
-                                      (* NOTE: if i will be scheduled arbitrary number of times, need recursive definition *)
-                                      ∨ False) (1/2)%Qp)
-               (1/2)%Qp
-    )%I.
+      VMProp_unknown ps_acc p_rx trans)%I.
 
 End logrel.
 
