theories/rules/mov.v
@@ -8,19 +8,20 @@ Section mov.
 Context `{hypparams: HypervisorParameters}.
 Context `{vmG: !gen_VMG Σ}.
 
-Lemma mov_word {E i w1 w3 q} a w2 ra :
+Lemma mov_word {E i w1 w3 q s} a w2 ra :
   decode_instruction w1 = Some (Mov ra (inl w2)) ->
+  (tpa a) ∈ s ->
   {SS{{ ▷ (PC @@ i ->r a)
         ∗ ▷ (a ->a w1)
-        ∗ ▷ (i -@{ q }A> (tpa a))
+        ∗ ▷ (i -@{ q }A> [s])
         ∗ ▷ (ra @@ i ->r w3)}}}
     ExecI @ i ; E
   {{{ RET (false, ExecI);  (PC @@ i ->r (a ^+ 1)%f)
                            ∗ (a ->a w1)
-                           ∗ (i -@{ q }A> (tpa a))
+                           ∗ (i -@{ q }A> [s])
                            ∗ ra @@ i ->r w2 }}}.
 Proof.
-  iIntros (Hdecode ϕ) "( >Hpc & >Hapc & >Hacc & >Hra) Hϕ".
+  iIntros (Hdecode Hin ϕ) "( >Hpc & >Hapc & >Hacc & >Hra) Hϕ".
   iApply (sswp_lift_atomic_step ExecI);[done|].
   iIntros (n σ1) "%Hsche Hσ".
   rewrite /scheduled in Hsche.
@@ -39,7 +40,6 @@ Proof.
   iDestruct ((gen_reg_valid2 i PC a ra w3 Hcur) with "Hreg Hpc Hra") as "[%HPC %Hra]".
   (* valid pt *)  
   iDestruct (access_agree_check_true _ i with "Haccess Hacc") as %Hacc;eauto.
-  { apply elem_of_singleton. reflexivity. }
   (* valid mem *)
   iDestruct (gen_mem_valid a w1 with "Hmem Hapc") as "%Hmem".
   iSplit.
@@ -118,21 +118,22 @@ Proof.
       intros Q; symmetry in Q; inversion Q; contradiction.
     Qed.
 
-Lemma mov_reg {E i w1 w3 q} a w2 ra rb :
+Lemma mov_reg {E i w1 w3 q s} a w2 ra rb :
   decode_instruction w1 = Some (Mov ra (inr rb)) ->
+  (tpa a) ∈ s ->
   {SS{{  ▷ (PC @@ i ->r a)
          ∗ ▷ (a ->a w1)
-         ∗ ▷ (i -@{ q }A> (tpa a))
+         ∗ ▷ (i -@{ q }A> [s])
          ∗ ▷ (ra @@ i ->r w2)
          ∗ ▷ (rb @@ i ->r w3) }}}
     ExecI @ i ;E
   {{{ RET (false, ExecI); PC @@ i ->r (a ^+ 1)%f
                    ∗ a ->a w1
-                   ∗ (i -@{ q }A> (tpa a))
+                   ∗ (i -@{ q }A> [s])
                    ∗ ra @@ i ->r w3
                    ∗ rb @@ i ->r w3}}}.
 Proof.
-  iIntros (Hdecode ϕ) "(>Hpc & >Hapc & >Hacc & >Hra & >Hrb) Hϕ".
+  iIntros (Hdecode Hin ϕ) "(>Hpc & >Hapc & >Hacc & >Hra & >Hrb) Hϕ".
   iApply (sswp_lift_atomic_step ExecI);[done|].
   iIntros (n σ1) "%Hsche Hσ".
   rewrite /scheduled in Hsche.
@@ -152,7 +153,6 @@ Proof.
   iDestruct ((gen_reg_valid3 i PC a ra w2 rb w3 Hcur) with "Hreg Hpc Hra Hrb") as "[%HPC [%Hra %Hrb]]".
   (* valid pt *)
   iDestruct (access_agree_check_true _ i with "Haccess Hacc") as %Hacc;eauto.
-  { apply elem_of_singleton. reflexivity. }
   (* valid mem *)
   iDestruct (gen_mem_valid a w1 with "Hmem Hapc") as "%Hmem".
   iSplit.
